Given categories \Cat\ and \Dat, and a functor $F:\Cat\to\Dat$, we saw
in proposition~(\ref{Fun:prop:opposite}) that $F$ is also a functor 
$F:\Cop\to\Dop$. Now consider two functors $F,G:\Cat\to\Dat$ and a natural 
transformation $\alpha:F \Rightarrow G$. By virtue of 
notation~(\ref{Nat:notation:natural:arrow}), $\alpha$ is a natural 
transformation between the typed functors $(\Cat,\Dat,F)$ and $(\Cat,\Dat,G)$, 
which are clearly understood from the context. But the notation is nonetheless 
ambiguous as it could also indicate that $\alpha$ is a natural
transformation between $(\Cop,\Dop,F)$ and $(\Cop,\Dop,G)$ among others. 
The two statements are not identical and in fact as it turns out, we
have the equivalence:

\begin{prop}
    Let $F,G:\Cat\to\Dat$ be functors between categories \Cat, \Dat. Then: 
    \[
        \alpha\,:\,(\Cat,\Dat,F)\,\Rightarrow\,(\Cat,\Dat,G)
    \]
    is equivalent to:
    \[
        \alpha\,:\,(\Cop,\Dop,G)\,\Rightarrow\,(\Cop,\Dop,F)
    \]
    In other words, being a natural transformation $\alpha:F\Rightarrow G$ (w.r.
    to \Cat\ and \Dat) is equivalent to being a natural transformation 
    $\alpha:G\Rightarrow F$ (w.r. to \Cop\ and \Dop):
    \begin{eqnarray}
        \begin{tikzcd}
            \Cat \arrow[r, "F", bend left  = 50, ""{name=U, below}]
                 \arrow[r, swap, "G", bend right = 50, ""{name=D, above}]
              & \Dat
            \arrow[Rightarrow, "\,\alpha", from = U, to = D]
        \end{tikzcd}
        &\Leftrightarrow&
        \begin{tikzcd}
            \Cop \arrow[r, "G", bend left  = 50, ""{name=U, below}]
                 \arrow[r, swap, "F", bend right = 50, ""{name=D, above}]
              & \Dop
            \arrow[Rightarrow, "\,\alpha", from = U, to = D]
        \end{tikzcd}
    \end{eqnarray}
\end{prop}
\begin{proof}
    from proposition~(\ref{Cat:prop:opposite:opposite}) we have
    $(\Cop)^{op}=\Cat$ and $(\Dop)^{op}=\Dat$ and it is therefore sufficient 
    to prove the implication $\Rightarrow$. So we assume that $\alpha$ is 
    a natural transformation $\alpha:(\Cat,\Dat,F)\Rightarrow(\Cat,\Dat,G)$,
    and we need to show that it is also a natural transformation
    $\alpha:(\Cop,\Dop,G)\Rightarrow(\Cop,\Dop,F)$. Looking at 
    definition~(\ref{Nat:def:natural}), we first need to establish that
    $\alpha$ is a map $\alpha:\ob\ \Cop\to\arr\ \Dop$. However, it is 
    certainly a map $\alpha:\ob\ \Cat\to\arr\ \Dat$ by assumption and from 
    definition~(\ref{Cat:def:opposite}) we have $\ob\ \Cat=\ob\ \Cop$ and
    $\arr\ \Dat=\arr\ \Dop$. Next we need to show property $(1)$ of
    definition~(\ref{Nat:def:natural}), namely that 
    $\alpha(a):G(a)\to F(a)\ @\ \Dop$ for all $a\in\ob\ \Cop$. This
    follows immediately from the fact that $\alpha(a):F(a)\to G(a)\ @\ \Dat$
    for all $a\in\ob\ \Cat$. So it remains to show property~$(2)$ of 
    definition~(\ref{Nat:def:natural}). So we assume that $a,b\in\ob\ \Cop
    =\ob\ \Cat$ and $f:a\to b\ @\ \Cop$. We need to show that 
    $F(f)\circ\alpha(a)\ @\ \Dop = \alpha(b)\circ G(f)\ @\ \Dop$, i.e.
    the following square commutes:
    \begin{eqnarray*}@\ \Cop
        &\begin{tikzcd}
            a\arrow[d,swap, "f"]
            &G(a)\arrow[r, "\alpha(a)"]\arrow[d, swap,"G(f)"]
            &F(a)\arrow[d, "F(f)"]
            \\
            b
            &G(b)\arrow[r, swap, "\alpha(b)"]
            &F(b)
        \end{tikzcd}&@\ \Dop
    \end{eqnarray*}
    A formal proof goes as follows: TODO
\end{proof}

