Let $T:\Bat\to\Cat$ and $F,G:\Cat\to\Dat$ be functors where \Bat, \Cat\
and \Dat\ are categories, and let $\alpha:F\Rightarrow G$ be a natural 
transformation. Then the situation is as follows: 
    \[
        \begin{tikzcd}
            \Bat \arrow[r,"T"]
            & \Cat \arrow[r, "F", bend left  = 50, ""{name=U, below}]
                 \arrow[r, swap, "G", bend right = 50, ""{name=D, above}]
              & \Dat
            \arrow[Rightarrow, "\,\alpha", from = U, to = D]
        \end{tikzcd}
    \] 
In particular the functors $F\circ T:\Bat\to\Dat$ and $G\circ T:\Bat\to\Dat$
are well-defined by virtue of definition~(\ref{Fun:def:composition}).
Furthermore, since $\alpha$ is a natural transformation $\alpha:F\Rightarrow G$,
using definition~(\ref{Nat:def:natural}), for all $a\in\Cat$ we have 
$\alpha(a):F(a)\to G(a)$. It follows that for all $a\in\Bat$ we have 
$\alpha (T(a)) : F(T(a))\to G(T(a))$. So the question arises as to whether
the expression $\alpha(T(a))$ for all $a\in\Bat$ defines a natural
transformation between $F\circ T$ and $G\circ T$. As we shall see the 
answer is 'yes' and we shall define a new natural transformation denoted 
$\alpha T$:
    \[
        \begin{tikzcd}
            \Bat \arrow[r,"T"]
            & \Cat \arrow[r, "F", bend left  = 50, ""{name=U, below}]
                 \arrow[r, swap, "G", bend right = 50, ""{name=D, above}]
              & \Dat
            \arrow[Rightarrow, "\,\alpha", from = U, to = D]
        \end{tikzcd}
        \ \to\ 
        \begin{tikzcd}
            \Bat \arrow[r, "F\circ T", bend left  = 50, ""{name=U, below}]
                 \arrow[r, swap, "G\circ T", bend right = 50, ""{name=D, above}]
              & \Dat
            \arrow[Rightarrow, "\,\alpha T", from = U, to = D]
        \end{tikzcd}
    \]

\begin{defin}\label{Nat:def:rightmul}
    Let $T:\Bat\to\Cat$ and $F,G:\Cat\to\Dat$ be functors where \Bat, \Cat\
    and \Dat\ are categories, and let $\alpha:F\Rightarrow G$ be a natural 
    transformation. We denote $\alpha T: F\circ T\Rightarrow G\circ T$ the 
    natural transformation defined by, given $a\in\ob\ \Bat$:
        \[
            (\alpha T)(a) = \alpha (T(a))
        \]
\end{defin}  

