module nat where

open import id    hiding (_+_)
open import bool
open import void
open import relations

data â„• : Set where
  zero : â„•
  succ : â„• â†’ â„•

{-# BUILTIN NATURAL â„• #-}

_+_ : â„• â†’ â„• â†’ â„•
zero   + y = y
succ x + y = succ (x + y)

succ-not-0 : (n : â„•) â†’ Â¬ (succ n â‰¡ 0)
succ-not-0 n ()

+-n+O : (n : â„•)â†’ n + 0 â‰¡ n
+-n+O zero     = refl 0
+-n+O (succ n) = ap succ (+-n+O n)

+-assoc : (n m p : â„•) â†’ (n + m) + p â‰¡ n + (m + p)
+-assoc zero m p     = refl (m + p)
+-assoc (succ n) m p = ap succ (+-assoc n m p)

+-n+succ : (n m : â„•) â†’ n + succ m â‰¡ succ (n + m)
+-n+succ zero m     = refl (succ m)
+-n+succ (succ n) m = ap succ (+-n+succ n m)

+-comm : (n m : â„•) â†’ n + m â‰¡ m + n
+-comm zero m     = â‰¡-sym (+-n+O m)
+-comm (succ n) m = â‰¡-trans (ap succ (+-comm n m)) (â‰¡-sym (+-n+succ m n))

infix 5 _+_
infix 6 _*_

_*_ : â„•Â â†’ â„• â†’ â„•
zero * m = 0
succ n * m = m + n * m

*-distribr : (n m p : â„•) â†’ (n + m) * p â‰¡ n * p + m * p
*-distribr zero m p     = refl (m * p)
*-distribr (succ n) m p = â‰¡-trans
  (ap (Î» x â†’ p + x) (*-distribr n m p))
  (â‰¡-sym (+-assoc p (n * p) (m * p)))

*-n*0 : (n : â„•) â†’ n * 0 â‰¡ 0
*-n*0 zero     = refl 0
*-n*0 (succ n) = *-n*0 n

*-n*succ : (n m : â„•) â†’ n * succ m â‰¡ n + n * m
*-n*succ zero m     = refl 0
*-n*succ (succ n) m = ap succ
  (â‰¡-trans
    (â‰¡-trans
      (â‰¡-trans
        (ap (Î» x â†’ m + x) (*-n*succ n m))
        (â‰¡-sym (+-assoc m n (n * m))))
      (ap (Î» x â†’ x + n * m) (+-comm m n)))
     (+-assoc n m (n * m)))


*-comm : (n m : â„•) â†’ n * m â‰¡ m * n
*-comm zero m     = â‰¡-sym (*-n*0 m)
*-comm (succ n) m = â‰¡-sym
  (â‰¡-trans
    (*-n*succ m n)
    (ap (Î» x â†’ m + x) (â‰¡-sym (*-comm n m)))) 


*-assoc : (n m p : â„•) â†’ (n * m) * p â‰¡ n * (m * p)
*-assoc zero m p     = refl 0
*-assoc (succ n) m p = â‰¡-trans
  (*-distribr m (n * m) p)
  (ap (Î» x â†’ m * p + x) (*-assoc n m p))

_=â„•_ : â„• â†’ â„• â†’ ğ”¹
zero =â„• zero     = tt
zero =â„• succ m   = ff
succ n =â„• zero   = ff
succ n =â„• succ m = n =â„• m

=â„•-refl : (n : â„•) â†’ (n =â„• n) â‰¡ tt
=â„•-refl zero     = refl tt
=â„•-refl (succ n) = =â„•-refl n

=â„•-sym : (n m : â„•) â†’ (n =â„• m) â‰¡ tt â†’ (m =â„• n) â‰¡ tt
=â„•-sym zero zero p         = refl tt
=â„•-sym (succ n) (succ m) p = =â„•-sym n m p

=â„•-trans : (n m p : â„•) â†’ (n =â„• m â‰¡ tt) â†’ (m =â„• p â‰¡ tt) â†’ (n =â„• p â‰¡ tt)
=â„•-trans zero zero zero q_nm q_mp = refl tt
=â„•-trans (succ n) (succ m) (succ p) q_nm q_mp = =â„•-trans n m p q_nm q_mp

=â„•-to-â‰¡ : (n m : â„•) â†’ (n =â„• m â‰¡ tt) â†’ n â‰¡ m
=â„•-to-â‰¡ zero zero p = refl zero
=â„•-to-â‰¡ (succ n) (succ m) p = ap succ (=â„•-to-â‰¡ n m p)

=â„•-from-â‰¡ : (n m : â„•) â†’ (n â‰¡ m) â†’ (n =â„• m â‰¡ tt)
=â„•-from-â‰¡ n m p = â‰¡-trans (â‰¡-sym (ap (Î» x â†’ n =â„• x) p)) (=â„•-refl n)

is-even : â„• â†’ ğ”¹
is-odd  : â„• â†’ ğ”¹
is-even zero = tt
is-even (succ n) = is-odd n
is-odd zero = ff
is-odd (succ n) = is-even n

data _â‰¤_ : â„• â†’ â„• â†’ Set where
  le-n : (n : â„•)   â†’ n â‰¤ n
  le-s : {n m : â„•} â†’ n â‰¤ m â†’ n â‰¤ succ m 

infixr 4 _â‰¤_

_<_ : â„• â†’ â„• â†’ Set
n < m = succ n â‰¤ m

â‰¤-refl : (n : â„•) â†’ n â‰¤ n
â‰¤-refl n = le-n n

â‰¤-trans : {n m p : â„•} â†’ n â‰¤ m â†’ m â‰¤ p â†’ n â‰¤ p
â‰¤-trans p (le-n n) = p
â‰¤-trans p (le-s q) = le-s (â‰¤-trans p q)

â‰¤-n-s : {n m : â„•} â†’ n â‰¤ m â†’ succ n â‰¤ succ m
â‰¤-n-s (le-n n) = le-n (succ n)
â‰¤-n-s (le-s p) = le-s (â‰¤-n-s p)

â‰¤-s-n : {n m : â„•} â†’ succ n â‰¤ succ m â†’ n â‰¤ m
â‰¤-s-n {n} {.n} (le-n .(succ n)) = le-n n
â‰¤-s-n {n} {m} (le-s p)          = â‰¤-trans (le-s (le-n n)) p

pred : (n : â„•) â†’ â„•
pred zero     = 0
pred (succ n) = n

<-n-s : {n m : â„•} â†’ n < m â†’ succ n < succ m
<-n-s p = â‰¤-n-s p 

<-s-n : {n m : â„•} -> succ n < succ m -> n < m
<-s-n p = â‰¤-s-n p

<-irrefl : {n : â„•} â†’ (n < n) -> ğ•†
<-irrefl {succ n} p = <-irrefl (<-s-n p) 

-- This is a weak result
<-trans : {n m p : â„•} â†’ n < m â†’ m < p â†’ n < p
<-trans {n} {m} {p} pnm qmp = â‰¤-trans pnm (â‰¤-trans (le-s (le-n m)) qmp)

â‰¤-transitive2 : transitive _â‰¤_
â‰¤-transitive2 = â‰¤-trans
