module list where

open import id
open import nat
open import bool
open import void
open import maybe

data ğ•ƒ {â„“} (a : Set â„“) : Set â„“ where
  []  : ğ•ƒ a
  _âˆ·_ : a â†’ ğ•ƒ a â†’ ğ•ƒ a

infixr 5 _âˆ·_

length :  âˆ€ {â„“} {a : Set â„“} â†’ ğ•ƒ a â†’ â„•
length []       = 0
length (x âˆ· xs) = succ (length xs)

_++_ : âˆ€ {â„“} {a : Set â„“} â†’ ğ•ƒ a â†’ ğ•ƒ a â†’ ğ•ƒ a
[] ++ ys       = ys
(x âˆ· xs) ++ ys = x âˆ· xs ++ ys

infixr 6 _++_

++[] : âˆ€ {â„“} â†’ {a : Set â„“} â†’ (xs : ğ•ƒ a) â†’ xs ++ [] â‰¡ xs
++[] []       = refl _
++[] (x âˆ· xs) = ap ((Î» l â†’ x âˆ· l)) (++[] xs)

++-[]-left : âˆ€ {â„“} â†’ {a : Set â„“} â†’ (xs ys : ğ•ƒ a) â†’ xs ++ ys â‰¡ [] â†’ xs â‰¡ []
++-[]-left [] _ _ = refl _

++-[]-right : âˆ€ {â„“} â†’ {a : Set â„“} â†’ (xs ys : ğ•ƒ a) â†’ xs ++ ys â‰¡ [] â†’ ys â‰¡ []
++-[]-right [] ys p = p

map : âˆ€ {â„“ â„“'} {a : Set â„“} {b : Set â„“'} â†’ (a â†’ b) â†’ ğ•ƒ a â†’ ğ•ƒ b
map f []       = []
map f (x âˆ· xs) = f x âˆ· map f xs

map-[] : âˆ€ {â„“ â„“'} â†’ {a : Set â„“} â†’ {b : Set â„“'} â†’ (f : a -> b) â†’ (xs : ğ•ƒ a) â†’
  map f xs â‰¡ [] â†’ xs â‰¡ []
map-[] _ [] _ = refl _

filter : âˆ€ {â„“} {a : Set â„“} â†’ (a â†’ ğ”¹) â†’ ğ•ƒ a â†’ ğ•ƒ a
filter p []       = []
filter p (x âˆ· xs) = let ys = filter p xs in if p x then x âˆ· ys else ys


remove : âˆ€ {â„“} {a : Set â„“} (eq : a â†’ a â†’ ğ”¹) (x : a) â†’ ğ•ƒ a â†’ ğ•ƒ a
remove eq a xs = filter (Î» x â†’ not (eq a x)) xs

nth : âˆ€ {â„“} {a : Set â„“} â†’ â„• â†’ ğ•ƒ a â†’ maybe a
nth _ []              = nothing
nth zero (x âˆ· _)      = just x
nth (succ n) (_ âˆ· xs) = nth n xs

-- inefficient
sreverse : âˆ€ {â„“} {a : Set â„“} â†’ ğ•ƒ a â†’ ğ•ƒ a
sreverse []       = []
sreverse (x âˆ· xs) = sreverse xs ++ (x âˆ· [])

reverse-go : âˆ€ {â„“} {a : Set â„“} â†’ ğ•ƒ a â†’ ğ•ƒ a â†’ ğ•ƒ a
reverse-go acc []       = acc
reverse-go acc (x âˆ· xs) = reverse-go (x âˆ· acc) xs

reverse : âˆ€ {â„“} {a : Set â„“} â†’ ğ•ƒ a â†’ ğ•ƒ a
reverse xs = reverse-go [] xs

{-
reverse_same : âˆ€ {â„“} {a : Set â„“} (xs : ğ•ƒ a) â†’ sreverse xs â‰¡ reverse xs
reverse [] same     = refl []
reverse x âˆ· xs same = {!!}
-}

length-++ : âˆ€ {â„“} {a : Set â„“} (xs ys : ğ•ƒ a) â†’
  length (xs ++ ys) â‰¡ length xs + length ys
  
length-++ [] ys       = refl (length ys)
length-++ (x âˆ· xs) ys = ap succ (length-++ xs ys)

++-assoc : âˆ€ {â„“} {a : Set â„“} (xs ys zs : ğ•ƒ a) â†’ (xs ++ ys) ++ zs â‰¡ xs ++ (ys ++ zs)
++-assoc [] ys zs       = refl (ys ++ zs)
++-assoc (x âˆ· xs) ys zs = ap (Î» ls â†’ x âˆ· ls) (++-assoc xs ys zs)


length-filter : âˆ€ {â„“} {a : Set â„“} (p : a â†’ ğ”¹) (xs : ğ•ƒ a) â†’
  length (filter p xs) â‰¤ length xs
length-filter p []       = le-n 0
length-filter p (x âˆ· xs) with (p x)
length-filter p (x âˆ· xs) | tt = â‰¤-n-s (length-filter p xs)
length-filter p (x âˆ· xs) | ff = le-s (length-filter p xs)

filter-idempotent : âˆ€ {â„“} {a : Set â„“} (p : a â†’ ğ”¹) (xs : ğ•ƒ a) â†’
  (filter p (filter p xs)) â‰¡ filter p xs
filter-idempotent p []            = refl []
filter-idempotent p (x âˆ· xs) with inspect (p x)
filter-idempotent p (x âˆ· xs) | tt withâ‰¡ eq =
  â‰¡-trans -- should be using rewrite, but don't understand it
    (ap (Î» b â†’ filter p (if b then x âˆ· filter p xs else filter p xs)) eq)
    (â‰¡-trans
      (ap (Î» b â†’ if b then x âˆ· filter p (filter p xs) else filter p (filter p xs)) eq)
      (â‰¡-sym
        (â‰¡-trans
          (ap (Î» b â†’ if b then x âˆ· filter p xs else filter p xs) eq)
          (ap (Î» l â†’ x âˆ· l)
            (â‰¡-sym (filter-idempotent p xs))))))
filter-idempotent p (x âˆ· xs) | ff withâ‰¡ eq = â‰¡-trans
  ((ap (Î» b â†’ filter p (if b then x âˆ· filter p xs else filter p xs)) eq ))
    (â‰¡-sym
      (â‰¡-trans
        ((ap (Î» b â†’ if b then x âˆ· filter p xs else filter p xs) eq))
          (â‰¡-sym (filter-idempotent p xs))))

length-reverse-go : âˆ€ {â„“} {a : Set â„“} (acc xs : ğ•ƒ a) â†’
  length (reverse-go acc xs) â‰¡ length acc + length xs
length-reverse-go acc []       = â‰¡-sym (+-n+O (length acc))
length-reverse-go acc (x âˆ· xs) = â‰¡-trans
  (length-reverse-go (x âˆ· acc) xs)
  (â‰¡-sym (+-n+succ (length acc) (length xs)))

length-reverse : âˆ€ {â„“} {a : Set â„“} (xs : ğ•ƒ a) â†’ length (reverse xs) â‰¡ length xs
length-reverse xs = length-reverse-go [] xs


concat : âˆ€ {â„“} {a : Set â„“} (xss : ğ•ƒ (ğ•ƒ a)) â†’ ğ•ƒ a
concat []           = []
concat (xs âˆ· xss)   = xs ++ concat xss

