\begin{defin}\label{Cat:def:homset}
    Let \Cat\ be a category and $a,b\in\Cat$. We call {\em hom-set of \Cat\ 
    associated with the ordered pair $(a,b)$} the collection denoted $\Cat(a,b)$ 
    and defined as:
        \[
            \Cat(a,b) = \{\ f\in\arr\ \Cat\ |\ f : a \to b\ \}
        \]
\end{defin}

\noindent
In other words the collection $\Cat(a,b)$ is the collection of all arrows $f$ in
\Cat\ such that $\dom(f)=a$ and $\cod(f)=b$. Note that despite being called a
'hom-set', the collection $\Cat(a,b)$ is generally not a set but an 
arbitary collection.

\begin{prop}\label{Cat:prop:homset:opposite}
    Let \Cat\ be a category and $a,b\in\Cat$. Then $\Cop(a,b)=\Cat(b,a)$.
\end{prop}
\begin{proof}
    Denoting $\dom'=\cod$ and $\cod'=\dom$ we have:
        \begin{eqnarray*}\Cop(a,b)
            &=&\{\ f\in\arr\ \Cop\ |\ f : a \to b\ @~\Cop\ \}\\
            \mbox{def.~(\ref{Cat:def:opposite})\ $\to$\ }
            &=&\{\ f\in\arr\ \Cat\ |\ f : a \to b\ @~\Cop\ \}\\
            \mbox{def.~(\ref{Cat:def:opposite})\ $\to$\ }
            &=&\{\ f\in\arr\ \Cat\ |\ \dom'(f)=a\ ,\ \cod'(f)=b\ \}\\
            &=&\{\ f\in\arr\ \Cat\ |\ \cod(f)=a\ ,\ \dom(f)=b\ \}\\
            &=&\{\ f\in\arr\ \Cat\ |\ f : b \to a\ @~\Cat\ \}\\
            &=&\Cat(b,a)
        \end{eqnarray*}
\end{proof}

\begin{prop}\label{Cat:prop:homset:product}
    Let \Cone, \Ctwo\ be two categories and $a,b\in\Cone\times\Ctwo$. Then:
        \[
            \Cone\times\Ctwo\,(a,b) 
            = 
            \Cone(a_{1},b_{1})\times\Ctwo(a_{2},b_{2})
        \]
    where it is understood that $a=(a_{1},a_{2})$ and $b=(b_{1},b_{2})$.
\end{prop}
\begin{proof}
    Let $a=(a_{1},a_{2})$ and $b=(b_{1},b_{2})$ be objects in the
    product category $\Cone\times\Ctwo$:
    \begin{eqnarray*}\Cone\times\Ctwo\,(a,b) 
        &=&\Cone\times\Ctwo\,[\,(a_{1},a_{2})\,,\,(b_{1},b_{2})\,]\\
        \mbox{def.~(\ref{Cat:def:homset})\ $\to$\ }
        &=&\{\ f\in\arr\ (\Cone\times\Ctwo)\ \ |\ \ 
               f : (a_{1},a_{2})\to(b_{1},b_{2})\ \}\\
        \mbox{def.~(\ref{Cat:def:canonical:product})\ $\to$\ }
        &=&\{\ (f_{1},f_{2})\ |\ f_{1}\in\arr\ \Cone\ ,\ f_{2}\in\arr\ \Ctwo\\
        &\ &\,,\ (f_{1},f_{2}) : (a_{1},a_{2})\to(b_{1},b_{2})\ \}\\
        &=&\{\ (f_{1},f_{2})\ |\ f_{1}\in\arr\ \Cone\ ,\ f_{2}\in\arr\ \Ctwo\\
        &\ &\,,\ \dom(f_{1},f_{2})=(a_{1},a_{2})\\
        &\ &\,,\ \cod(f_{1},f_{2})=(b_{1},b_{2})\ \}\\
        \mbox{$(3)$ and $(4)$ of def.~(\ref{Cat:def:canonical:product})\ $\to$\ }
        &=&\{\ (f_{1},f_{2})\ |\ f_{1}\in\arr\ \Cone\ ,\ f_{2}\in\arr\ \Ctwo\\
        &\ &\,,\ (\,\dom(f_{1})\,,\,\dom(f_{2})\,)=(a_{1},a_{2})\\
        &\ &\,,\ (\,\cod(f_{1})\,,\,\cod(f_{2})\,)=(b_{1},b_{2})\ \}\\
        &=&\{\ (f_{1},f_{2})\ |\ f_{1}\in\arr\ \Cone\ ,\ f_{2}\in\arr\ \Ctwo\\
        &\ &\,,\ f_{1}:a_{1}\to b_{1}\ ,\ f_{2}:a_{2}\to b_{2}\ \}\\
        \mbox{product of collections\ $\to$\ }
        &=&\{\ f_{1}\in\arr\ \Cone\ |\ f_{1}:a_{1}\to b_{1}\ \}\\
        &\times& \{\ f_{2}\in\arr\ \Ctwo\ |\ f_{2}:a_{2}\to b_{2}\ \}\\
        \mbox{def.~(\ref{Cat:def:homset})\ $\to$\ }
        &=&\Cone(a_{1},b_{1})\times\Ctwo(a_{2},b_{2})
    \end{eqnarray*}
\end{proof}

\begin{prop}\label{Cat:prop:homset:set}
    For all sets $a,b$, the hom-set $\Set(a,b)$ is given by:
        \[
            \Set(a,b)=\{\ (a,b,f)\ |\ 
            \mbox{f is a function $f:a\to b$}\ \}
        \]
\end{prop}
\begin{proof}
    \begin{eqnarray*}\Set(a,b)
        &=&\{\ f\in\arr\ \Set\ |\ f : a \to b\ \}
        \ \leftarrow\ \mbox{def.~(\ref{Cat:def:homset})}\\
        \mbox{notation~(\ref{Cat:notation:arrow:a:b})}\ \to\ 
        &=&\{\ f\in\arr\ \Set\ |\ \dom(f)=a\ ,\ \cod(f)=b\  \}\\
        \mbox{$(2)$ of def.~(\ref{Cat:def:set})}\ \to\ 
        &=&\{\ (x,y,f)\ |\ x,y\ \mbox{sets, f is a function 
        $f:x\to y$}\\
        &\ &,\ \dom(x,y,f)=a\ ,\ \cod(x,y,f)=b\ \}\\
        \mbox{$(3)$ and $(4)$ of def.~(\ref{Cat:def:set})}\ \to\ 
        &=&\{\ (x,y,f)\ |\ x,y\ \mbox{sets, f is a function 
        $f:x\to y$}\\
        &\ &,\ x=a\ ,\ y=b\ \}\\
        &=&\{\ (a,b,f)\ |\ \mbox{f is a function $f:a\to b$}\ \}
    \end{eqnarray*}
\end{proof}
