\begin{defin}\label{logic:def:LAM:substitution}
    Let $V$ and $W$ be two sets and $\sigma:V\to W$ be a map. We call
    {\em substitution mapping between \tv\ and ${\bf T}(W)$ associated
    with $\sigma:V\to W$} the map $\sigma^{*}:\tv\to{\bf T}(W)$ defined
    by the structural recursion:
    \begin{equation}\label{logic:eqn:LAM:substitution:recursion}
        \forall\phi\in\tv\ ,\ \sigma^{*}(\phi)=\left\{
            \begin{array}{lcl}
                \sigma(x)
                    &\mbox{\ if\ }&
                \phi=x
                \\
                \sigma^{*}(\phi_{1})\ \sigma^{*}(\phi_{2}) 
                    &\mbox{\ if\ }&
                \phi=\phi_{1}\ \phi_{2}
                \\
                \lambda\sigma(x)\,\sigma^{*}(\phi_{1})
                    &\mbox{\ if\ }&
                \phi=\lambda x\phi_{1}
            \end{array}\right.
    \end{equation}
\end{defin}

\begin{prop}\label{logic:prop:LAM:substitution}
    The structural recursion of 
    {\em definition~(\ref{logic:def:LAM:substitution})} 
    is legitimate.
\end{prop}
\begin{proof}
    TODO
\end{proof}

\begin{prop}\label{logic:prop:LAM:substitution:composition}
    Let $U$, $V$ and $W$ be sets. Let $\tau:U\to V$ and $\sigma:V\to W$
    be maps. Let $\tau^{*}:{\bf T}(U)\to\tv$ and $\sigma^{*}:\tv\to{\bf
    T}(W)$ be the substitution mappings associated with $\tau$ and
    $\sigma$ respectively. Then:
    \[
        (\sigma\circ\tau)^{*}
        =
        \sigma^{*}\circ\tau^{*}
    \]
    where $(\sigma\circ\tau)^{*}:{\bf T}(U)\to {\bf T}(W)$ is the
    substitution mapping associated with $\sigma\circ\tau$.
\end{prop}
\begin{proof}
    TODO
\end{proof}

\begin{prop}\label{logic:prop:LAM:substitution:identity}
    Let $V$ be a set and $i:V\to V$ be the identity mapping. Then, the
    associated substitution mapping $i:\tv\to\tv$ is also the identity.
\end{prop}
\begin{proof}
    TODO
\end{proof}

\begin{prop}\label{logic:prop:LAM:substitution:subformula}
Let $V,W$ be sets and $\sigma:V\to W$ be a map. The associated
substitution $\sigma:\tv\to{\bf T}(W)$ is a structural substitution
and for all $\phi\in\tv$\,:
    \[
        \subf(\sigma(\phi))
        =
        \sigma(\subf(\phi))
    \]
\end{prop}
\begin{proof}
    TODO
\end{proof}

