\begin{defin}\label{Fun:def:constant}
    Let \Cat,\ \Dat\ be categories and $d\in\Dat$. We call {\em constant functor 
    from \Cat\ to \Dat\ at $d$} the functor $F:\Cat\to\Dat$ defined by 
    $F=(F_{0},F_{1})$ with:
        \begin{eqnarray*}
            (1)&\ &F_{0}(c) = d\\
            (2)&\ &F_{1}(f) = \id(d)
        \end{eqnarray*}
    where $(1)$ holds for all $c\in\ob\ \Cat$ and $(2)$ holds for all
    $f\in\arr\ \Cat$.
\end{defin}

\begin{notation}\label{Fun:notation:constant}
    The constant functor from \Cat\ to \Dat\ at $d\in\Dat$ is denoted $K_{d}$.
\end{notation}

\noindent
{\bf Remark}: The notation $K_{d}$ is ambiguous and must be understood in a context.

\noindent
We shall now check our definition is indeed that of a functor.

\begin{prop}\label{Fun:prop:constant}
    Given categories \Cat,\ \Dat\ and $d\in\Dat$, $K_{d}$ is a functor $K_{d}:
    \Cat\to\Dat$.
\end{prop}
\begin{proof}
    Let \Cat,\ \Dat\ be categories, $d\in\Dat$ and $K_{d}=(F_{0},F_{1})$ be the 
    constant functor from \Cat\ to \Dat\ at $d$. We need to check properties 
    $(1)-(5)$ of definition~(\ref{Fun:def:functor}):

    $(1)$: $F_{0}$ is indeed a map $F_{0}:\ob\ \Cat \to\ob\ \Dat$ from $(1)$ 
    of definition~(\ref{Fun:def:constant}).

    $(2)$: $F_{1}$ is indeed a map $F_{1}:\arr\ \Cat\to\arr\ \Dat$ from $(2)$ 
    of definition~(\ref{Fun:def:constant}).

    $(3)$: We have $F_{1}(f):F_{0}(a)\to F_{0}(b)$ whenever $f:a\to b$, since:
        \[
            F_{1}(f)=\id(d),\  F_{0}(a)=d,\ F_{0}(b)=d
        \]

    $(4)$: We have $F_{1}(\,\id(a)\,)=\id(\,F_{0}(a)\,)$ for
    all $a\in\Cat$, since:
        \[
            F_{1}(\,\id(a)\,)=\id(d),\ F_{0}(a)=d
        \]

    $(5)$: $F_{1}(g\circ f)=F_{1}(g)\circ F_{1}(f)$ whenever $f:a\to b$ 
    and $g:b\to c$, since:
        \[
            F_{1}(g\circ f) = \id(d),\ F_{1}(g)=\id(d),\  F_{1}(f)=\id(d)
        \]
    and $\id(d)=\id(d)\circ\id(d)$ from $(12)$ (or $(13)$) of
    definition~(\ref{Cat:def:category}).
\end{proof}
