\begin{defin}\label{Fun:def:identity}
    Let \Cat\ be a category. We call {\em identity functor on} \Cat\ the 
    functor $F:\Cat\to\Cat$ defined by $F=(F_{0},F_{1})$ with:
        \begin{eqnarray*}
            (1)&\ &F_{0}(a) = a\\
            (2)&\ &F_{1}(f) = f
        \end{eqnarray*}
    where $(1)$ holds for all $a\in\ob\ \Cat$ and $(2)$ holds for all
    $f\in\arr\ \Cat$.
\end{defin}

\begin{notation}\label{Fun:notation:identity}
    The identity functor on a category \Cat\ is denoted $I_{\cal C}$.
\end{notation}

\noindent
We shall now check our definition is indeed that of a functor.

\begin{prop}\label{Fun:prop:identity}
    The identity functor on a category \Cat\ is a functor $I_{\cal C}:
    \Cat\to\Cat$.
\end{prop}
\begin{proof}
    Let \Cat\ be a category and $I_{\cal C}=(F_{0},F_{1})$ be the identity
    functor on \Cat. We need to check that properties $(1)-(5)$ of
    definition~(\ref{Fun:def:functor}) are satisfied:

    $(1)$: $F_{0}$ is indeed a map $F_{0}:\ob\ \Cat \to\ob\ \Cat$ from $(1)$ 
    of definition~(\ref{Fun:def:identity}).

    $(2)$: $F_{1}$ is indeed a map $F_{1}:\arr\ \Cat\to\arr\ \Cat$ from $(2)$ 
    of definition~(\ref{Fun:def:identity}).

    $(3)$: We have $F_{1}(f):F_{0}(a)\to F_{0}(b)$ whenever $f:a\to b$, since:
        \[
            F_{1}(f)=f,\ F_{0}(a)=a,\ F_{0}(b)=b
        \]

    $(4)$: We have $F_{1}(\,\id(a)\,)=\id(\,F_{0}(a)\,)$ for
    all $a\in\Cat$, since: 
        \[
            F_{1}(\,\id(a)\,)=\id(a),\ F_{0}(a)=a
        \]

    $(5)$: $F_{1}(g\circ f)=F_{1}(g)\circ F_{1}(f)$ whenever $f:a\to b$ 
    and $g:b\to c$, since:
        \[
            F_{1}(g\circ f) = g\circ f,\ F_{1}(g)=g,\  F_{1}(f)=f
        \]
\end{proof}
